some attempts at mutating for_each

mutating_map.v
@@ -11,13 +11,16 @@ Fixpoint is_list `{!heapG Σ} (v : val) (Ψs : list (val -> iProp Σ)) : iProp �
   | Ψ :: Ψs' => ∃(lh : loc) (x vt : val), ⌜v = InjRV #lh⌝ ∗ lh ↦ (x, vt) ∗ Ψ x ∗ is_list vt Ψs'
 end%I.
 
+Definition list_const {Σ} (xs : list val) : list (val -> iProp Σ) :=
+  (map (fun x v => ⌜v = x⌝%I) xs).
+
 Section MutatingMap.
   Context `{heapG Σ}.
 
   Definition prog_mktestlist : val := λ: "unit",
-    let: "x" := ref #3 in
-    let: "cons" := ref ("x", InjL #()) in
-    InjR "cons".
+                                      let: "x" := ref #3 in
+                                      let: "cons" := ref ("x", InjL #()) in
+                                      InjR "cons".
 
   Definition points_to_three (v : val) : iProp Σ :=
     (∃(l : loc), ⌜v = #l⌝ ∗ l ↦ #3)%I.
@@ -29,13 +32,91 @@ Section MutatingMap.
     wp_alloc lc1 as "H1". wp_pures.
     wp_alloc lc2 as "H2". wp_pures.
     rewrite /is_list /points_to_three.
-    iExists lc2.
-    iExists (#lc1)%V.
-    iExists (InjLV #())%V.
+    iExists lc2, #lc1, (InjLV #()).
     iFrame.
     iSplitR. done.
     iSplitL. iExists lc1. iFrame. done.
     done.
+  Qed.
+
+  Definition closure_test : expr :=
+    let: "s" := ref #0 in
+    let: "f" := λ: "x", "s" <- !"s" + "x" in
+    "f" #1;; !"s".
+
+  Lemma closure_test_wp:
+    WP closure_test {{ v, ⌜v = #1⌝ }}%I.
+  Proof.
+    iIntros "".
+    rewrite /closure_test.
+    wp_alloc ls as "Hs".
+    by repeat (wp_load || wp_store || wp_pure _).
+  Qed.
+
+  Definition prog_for_each : val :=
+    rec: "for_each" "f" "xs" :=
+      match: "xs" with
+        InjL "unit" => Skip
+      | InjR "cons" => "f" (Fst !"cons");; "for_each" (Snd !"cons")
+      end.
+
+  Lemma prog_for_each_wp
+        (v : val)
+        (Ψs : list (val -> iProp Σ))
+        (I : list val -> iProp Σ)
+        (f : val)
+        (T : (val -> iProp Σ) -> (val -> iProp Σ)):
+    {{{ is_list v Ψs
+      ∗ I []
+      ∗ ∀ x xs Ψ, {{{ Ψ x ∗ I xs }}} f x {{{ RET #(); T Ψ x ∗ I (x :: xs) }}}
+    }}}
+      prog_for_each f v
+    {{{ RET #(); is_list v (map T Ψs) }}}.
+  Proof.
+  Admitted.
+
+  Definition prog_sum : val := λ: "xs",
+    let: "s" := ref #0 in
+    let: "f" := λ: "x", "s" <- !"s" + !"x";; "x" <- !"x" + #1 in
+    prog_for_each "f" "xs";; !"s".
+
+  (* This is what the closure looks like after some beta
+  reductions. There are not actually any free variables on the object
+  language level. *)
+  Definition prog_increment_closure (ls : loc) : val :=
+    λ: "x", #ls <- !#ls + !"x";; "x" <- !"x" + #1.
+
+  Definition nums_to_vals (xs : list Z) : list val := map (fun x : Z => #x) xs.
+
+  Definition loop_invariant (ls : loc) (xs : list val) : iProp Σ :=
+    (∃(xs' : list Z), ⌜xs = nums_to_vals xs'⌝ ∗ ls ↦ #(fold_right Z.add 0 xs'))%I.
+
+  (* Idea: you should not be able to assume that the list will be
+  processed in any particular order in the mapping function that is
+  supplied as the argument. *)
+  Lemma prog_sum_wp (v : val) (xs : list Z):
+    {{{ is_list v (list_const (nums_to_vals xs)) }}}
+      prog_sum v
+    {{{ r, RET r; is_list v (list_const (nums_to_vals (map (fun x => x + 1) xs))) ∗ ⌜r = #(fold_right Z.add 0 xs)⌝ }}}.
+  Proof.
+    iIntros (Φ) "Hv HΦ".
+    wp_rec. wp_alloc ls as "Hs". wp_pures.
+    wp_apply (prog_for_each_wp
+                v
+                (list_const (nums_to_vals xs))
+                (loop_invariant ls) _ _).
+  Admitted.
+
+  (* This is probably a strong enough specification of the
+  incrementing closure to be used in the application of for_each. *)
+  Lemma prog_increment_closure_wp (ls : loc) (lx : loc) (n : Z) (k : Z):
+    {{{ ls ↦ #n ∗ lx ↦ #k }}}
+      prog_increment_closure ls #lx
+    {{{ RET #(); ls ↦ #(n + k) ∗ lx ↦ #(k + 1) }}}.
+  Proof.
+    iIntros (Φ) "[Hls Hlx] HΦ".
+    wp_rec. repeat (wp_load || wp_store || wp_pure _).
+    iApply "HΦ". by iFrame.
   Qed.
 
 End MutatingMap.
